example/Pump.Extract.fst
@@ -1,27 +1,25 @@
 (* Compiling a simple example to C.
-   The program to translate is defined in Example.Check.Pump. *)
-module Example.Compile.Pump
+   The program to translate is defined in Pump.Check.fst. *)
+module Pump.Extract
 
-module Pump = Example.Check.Pump
+module Pump = Pump.Check
 
-module Exp = Pipit.Exp
 module XX  = Pipit.Exec.Exp
 module XL  = Pipit.Exec.LowStar
 
 module Tac = FStar.Tactics
-module B   = LowStar.Buffer
-open FStar.HyperStack.ST
 
-module Sugar = Pipit.SugarX4
+module Sugar = Pipit.Sugar
 
-(* We will translate the controller node with variables as input.
-   We do not want the expression's internal representation to show up in the
-   C code, so we mark it as noextract. *)
+(* We will translate just the controller node with two input streams (estop and
+   level). We do not want the expression's internal representation to show up in
+   the C code, so we mark it as noextract. *)
 noextract
 let expr = Sugar.run2 Pump.controller'
 
 (* Define the state type so it shows up as a type definition in the C code.
-   The "postprocess_with" annotation ensures that the state_of_exp is inlined into the type and simplified to a regular type *)
+   The "postprocess_with" annotation ensures that the state_of_exp is inlined
+   into the type and simplified to a regular type *)
 [@@(Tac.postprocess_with XL.tac_extract)]
 let state = XX.state_of_exp expr
 
@@ -33,7 +31,6 @@ type input = {
 (* Translate the expression to a transition system. *)
 noextract
 let system: Pipit.Exec.Exp.xexec expr =
-  // assert_norm (Exp.wf expr 2);
   assert_norm (XX.extractable expr);
   XX.exec_of_exp expr
 
@@ -43,14 +40,6 @@ let system: Pipit.Exec.Exp.xexec expr =
 let reset = XL.mk_reset system
 
 (* Define the step function, which takes two input integers and a pointer to the
-   internal state, and returns the result as a bitfield. We parse the bitfield
-   before returning the values.
-   *)
-
+   internal state, and returns the result as a pair. *)
 [@@(Tac.postprocess_with XL.tac_extract)]
 let step (inp: input) = XL.mk_step system (inp.estop, (inp.level_low, ()))
-
-// let step' (inp: input) (stref: B.pointer state): ST _
-//     (requires (fun h -> B.live h stref))
-//     (ensures (fun h _ h' -> B.live h' stref)) =
-//   step inp stref
