src/Pipit.Tactics.fst
@@ -1,0 +1,99 @@
+(* Helper tactics for simplifying Pipit expressions.
+   The tactics here are very simple. They just help to massage the transition
+   systems in Pipit.System.Exp into a nicer form for the SMT solver. *)
+module Pipit.Tactics
+
+module T = FStar.Tactics
+
+(* Re-exports *)
+let norm_full () = T.norm [delta; nbe; zeta; iota; primops]
+
+let dump s = T.dump s
+
+let dump_ () = dump "-"
+
+(* Check if a type is a tuple or unit type that we want the tactics to break
+   apart. *)
+let rec type_is_product (ty: T.typ): T.Tac bool =
+  match T.inspect_unascribe ty with
+  | T.Tv_FVar fv | T.Tv_UInst fv _ ->
+    let nm = T.inspect_fv fv in
+    begin
+      match nm with
+      | ["FStar"; "Pervasives"; "Native"; tt ] ->
+        tt <> "option"
+      // | ["Prims"; "unit"] ->
+      //  true
+      // See Pipit.System.Base.fst.
+      | ["Pipit"; "System"; "Base"; "system_then_state" ] ->
+        true
+      | _ -> false
+    end
+  | T.Tv_App f _ -> type_is_product f
+  | T.Tv_Const T.C_Unit -> true
+  | _ ->
+    false
+
+(* Check if type is unit *)
+let type_is_unit (ty: T.typ): T.Tac bool =
+  match T.inspect_unascribe ty with
+  | T.Tv_FVar fv | T.Tv_UInst fv _ ->
+    let nm = T.inspect_fv fv in
+    begin
+      match nm with
+      | ["Prims"; "unit"] ->
+        true
+      | _ -> false
+    end
+  | _ ->
+    false
+
+(* Break apart any product types bound in `bs`. *)
+let rec tac_products (bs: list T.binder): T.Tac unit = match bs with
+ | [] -> ()
+ | b :: bs ->
+   let open T in
+   let open FStar.List.Tot in
+   let tm = T.binder_to_term b in
+   let ty = T.type_of_binder b in
+   if type_is_unit ty
+   then begin
+     (try clear b with | _ -> ());
+     tac_products bs
+   end
+   else if type_is_product ty
+   then begin
+    T.destruct tm;
+    let bs' = T.repeat T.intro in
+    T.rewrite_all_context_equalities bs';
+    T.norm [iota];
+    let _ = T.trytac (fun () ->
+      match List.Tot.rev bs' with
+      | breq :: _ -> rewrite breq; clear breq; clear b
+      | _ -> clear b
+    ) in
+    tac_products (bs' @ bs)
+   end
+   else begin
+    tac_products bs
+   end
+
+let tac_intros_smash (): T.Tac unit =
+  T.repeatseq (fun _ ->
+    let b = T.forall_intro () in
+    tac_products [b])
+
+(* Introduce foralls and try to simplify them *)
+let rec pipit_simplify' (n: nat): T.Tac unit =
+  match n with
+  | 0 -> ()
+  | _ ->
+    let open T in
+    norm_full ();
+    try
+        let b = forall_intro () in
+        tac_products [b];
+        pipit_simplify' (n - 1)
+    with _ -> ()
+
+let pipit_simplify (): T.Tac unit = pipit_simplify' 5
