readme.md
@@ -1,5 +1,92 @@
 # Pipit
 
-Pipit is (will be) a formalisation of a small Lustre-style reactive language in [F*](https://www.fstar-lang.org/).
-Reactive languages are generally useful for writing realtime control systems, but Pipit itself is not at a useful stage yet.
-I hope to be able to re-use F-star's proof automation (via SMT) for model-checking programs.
+Pipit is an embedded language for implementing and verifying *reactive systems*, such as the anti-lock braking system in a car, or the  [system that fills the water reservoir of your coffee machine](https://youtu.be/6IybbQFPOl8).
+Pipit is a research project and is in the early stages of development.
+
+Pipit is implemented in  [F*](https://www.fstar-lang.org/).
+The language is strongly inspired by Lustre.
+The verification system is inspired by the [Kind2 model checker](https://github.com/kind2-mc/kind2/) and related work.
+By embedding Pipit in a theorem prover, we aim to have an expressive language with a small verifiable core.
+Pipit reuses F\*'s proof automation for proving properties of programs.
+We also reuse F\*'s C code generation to generate real-time code.
+
+The Pipit library is in the `src` subdirectory and has four main pieces:
+* the source language, which provides some syntactic niceties for writing language (`Pipit.Sugar`);
+* the core expression language, which provides a bigstep semantics (`Pipit.Exp` and submodules);
+* transition systems, which is used for reasoning about programs (`Pipit.System` and submodules); and
+* executable systems, which are used for compiling to C code (`Pipit.Exec` and submodules).
+
+Programs written in the core language are translated to a transition system for verification; this translation is verified (it preserves semantics).
+The translation to executable systems preserves types, but is not yet verified to preserve semantics.
+The details of the formalisation and proofs are available in the [implementation notes](src/readme.md).
+
+There are examples available in the `example` subdirectory ([readme](example/readme.md)).
+
+## Dependencies and development
+
+Pipit requires F\* and Karamel for generating C code.
+Pipit indirectly requires [opam](https://opam.ocaml.org/), the OCaml package manager. 
+
+Pipit requires a recent development version of F\*; I usually install it from source, available at [FStar on github](https://github.com/FStarLang/FStar).
+(TODO: I am using version F* 2023.04.08~dev; test with a released version)
+
+Karamel can be installed from source at [karamel on github](https://github.com/FStarLang/karamel/).
+
+### Dependency installation
+
+The following script should set up an environment.
+Make sure you have [opam](https://opam.ocaml.org/) installed.
+Run this from the Pipit directory:
+
+``` sh
+# Create a directory for the build environment
+mkdir -p build/env; cd build/env
+
+# Create a local opam switch with OCaml 4.14
+opam switch create . 4.14.1
+
+# git clone https://github.com/FStarLang/karamel
+
+# Is it necessary to check out a specific commit of F*?
+# git clone https://github.com/FStarLang/FStar
+# cd FStar; git checkout 5a15885098c69006bb56ff2712534fe75a5fd839; cd ..
+
+# Tell opam to use the development version of F* (but don't install it yet)
+opam pin add fstar --dev-repo --no-action
+
+# Tell opam where to find the local repo for Karamel (and install it and F*)
+opam pin add karamel --dev-repo --yes
+```
+
+### IDE configuration
+
+When using an IDE (Emacs, VSCode), you might need to specify the exact version of FStar and Z3 binaries to use.
+
+
+#### VSCode
+
+There are a few VSCode extensions that provide different levels of F\* support; you should use [fstar-vscode-assistant](https://marketplace.visualstudio.com/items?itemName=FStarLang.fstar-vscode-assistant).
+
+You may need to tell VSCode the path of your F\* installation.
+Copy `template.fst.config.json` to `.fst.config.json` and modify it to include the path to `fstar.exe` as necessary.
+
+If you have multiple versions of Z3 installed, you will probably also have to specify the path to the F\*-compatible Z3 with the `--smt /.../bin/z3` option.
+For example, my `.fst.config.json` is:
+
+```json
+{ "fstar_exe":"/Users/amos/proj/ext/fstar/_opam/bin/fstar.exe",
+  "options":["--smt", "/Users/amos/proj/ext/fstar/_opam/bin/z3", "--cache_dir", ".cache.boot"],
+  "include_dirs":["src","example"]
+}
+```
+
+#### Emacs
+
+Emacs
+
+``` emacs-lisp
+(setq-default
+  fstar-executable "/Users/amos/proj/ext/fstar/_opam/bin/fstar.exe"
+  fstar-smt-executable "/Users/amos/proj/ext/fstar/_opam/bin/z3")
+```
+
